\documentclass[a4paper,17pt]{extarticle}
\usepackage[utf8]{inputenc}
\usepackage[left=8mm, top=0.5in]{geometry}

\begin{document}

$\beta \textbf{ - reduction of this } \lambda \textbf{ - term:}$ \newline

$((\lambda a.(\lambda b.b b) (\lambda b.b b)) b) ((\lambda c.(c b)) (\lambda a.a))$ \newline

$\textbf{1) } ((\lambda a.(\lambda b.b b) (\lambda b.b b)) b) ((\lambda c.(c b)) (\lambda a.a)) \Longrightarrow_\beta $ \newline

$\textbf{2) } ((\lambda b.b b)\ (\lambda b.b b)) ((\lambda c.(c b)) (\lambda a.a)) \Longrightarrow_\beta $ \newline

$\textbf{3) } ((\lambda b.b b)\ (\lambda b.b b)) ((\lambda a.a) b)) \Longrightarrow_\beta $ \newline

$\textbf{4) } ((\lambda b.b b)\ (\lambda b.b b)) b$ \newline

$\textbf{Answer: } ((\lambda b.b b)\ (\lambda b.b b))\ b$ 

\end{document}